pair-programming: starting map-swap example from Gallina

src/Examples/Incr/Incr.v
@@ -15,7 +15,12 @@ Require Import coqutil.Word.Interface coqutil.Word.Properties.
 Require Import coqutil.Map.Interface coqutil.Map.Properties.
 Require Import coqutil.Map.SortedList.
 Require Import coqutil.Tactics.destr.
+Require Import coqutil.Tactics.Tactics.
 Require Import Coq.Numbers.DecimalString.
+
+Require Import Rupicola.Examples.KVStore.KVStore.
+Require Import Rupicola.Examples.KVStore.Tactics.
+Require Import Rupicola.Examples.KVStore.Properties.
 
 Local Open Scope string_scope.
 Import ListNotations.
@@ -459,4 +464,209 @@ Module GallinaIncr.
     setup.
     repeat t.
   Qed.
+
+  Section KVSwap.
+    Context {ops} {key value : Type} {Value}
+            {dummy_value : value}
+            {kvp : kv_parameters}
+            {ok : @kv_parameters_ok ops key value Value kvp}.
+
+    Existing Instances ops kvp ok.
+    Existing Instances map_ok annotated_map_ok key_eq_dec.
+    Existing Instances spec_of_map_get spec_of_map_put.
+
+    Definition do_or_default {A B}
+               (a : option A) (f : A -> B) (default : B) : B :=
+      match a with
+      | Some a => f a
+      | None => default
+      end.
+
+    Notation "'let/o'  x  :=  val  'goto_fail' default 'in'  body" :=
+      (do_or_default val (fun x => body) default) (at level 4).
+
+    (* look up k1 and k2, add their values and store in k3 *)
+    Definition kvswap_gallina (m : map.rep (map:=map))
+               (k1 k2 : key) : map.rep (map:=map) * key * key :=
+      let/o v1 := map.get m k1 goto_fail (m, k1, k2) in
+      let/o v2 := map.get m k2 goto_fail (m, k1, k2) in
+      let/d m := map.put m k2 v1 in
+      let/d m := map.put m k1 v2 in
+      (m, k1, k2).
+
+    (*
+    Definition swap : bedrock_func :=
+      let m := "m" in
+      let k1 := "k1" in
+      let k2 := "k2" in
+      let v1 := "v1" in
+      let v2 := "v2" in
+      let err := "err" in
+      ("swap",
+       ([m; k1; k2], [],
+        bedrock_func_body:(
+          unpack! err, v1 = get (m, k1) ;
+            require !err ;
+            unpack! err, v2 = get (m, k2) ;
+            require !err ;
+            unpack! err = put (m, k2, v1)
+            (* now v2 is stored in v1 -- no need for second put *)
+      ))).
+     *)
+
+    Local Declare Scope sep_scope.
+    Local Delimit Scope sep_scope with sep.
+    Local Infix "*" := (sep) : sep_scope.
+    Definition MapAndTwoKeys pm pk1 pk2 v :=
+      let m := fst (fst v) in
+      let k1 := snd (fst v) in
+      let k2 := snd v in
+      (Map pm m * Key pk1 k1 * Key pk2 k2)%sep.
+
+    Definition deannotate (m : annotated_map) : map.rep (map:=map) :=
+      map.fold
+        (fun (m' : map.rep) (k : key) (v : annotation * value) =>
+           map.put m' k (snd v)) map.empty m.
+
+    Lemma get_deannotate_Some m k v :
+      map.get m k = Some v ->
+      map.get (deannotate m) k = Some (snd v).
+    Admitted.
+    Lemma get_deannotate_None m k :
+      map.get m k = None ->
+      map.get (deannotate m) k = None.
+    Admitted.
+
+    Lemma compile_map_get :
+      forall (locals: Semantics.locals) (mem: Semantics.mem)
+             tr R R' functions T (pred: T -> _ -> Prop)
+             m m_ptr m_var M
+             k k_ptr k_var
+             default default_impl
+             K K_impl,
+        spec_of_map_get functions ->
+        m = deannotate M ->
+      forall err var,
+        var <> err ->
+        (AnnotatedMap m_ptr M * Key k_ptr k * R')%sep mem ->
+        map.get locals m_var = Some m_ptr ->
+        map.get locals k_var = Some k_ptr ->
+        match map.get M k with
+        | None => True
+        | Some (Owned, _) => True
+        | _ => False
+        end ->
+        let v := (map.get m k) in
+        (forall head hd_ptr mem',
+            v = Some head ->
+            (AnnotatedMap m_ptr
+                          (map.put M k
+                                   (Reserved hd_ptr, head))
+             * Key k_ptr k * R')%sep mem' ->
+            find K_impl
+            implementing (pred (K head))
+            with-locals (map.put (map.put locals err (word.of_Z 0))
+                              var hd_ptr)
+            and-memory mem' and-trace tr and-rest R
+            and-functions functions) ->
+        (forall garbage mem',
+            v = None ->
+            (AnnotatedMap m_ptr M * Key k_ptr k * R')%sep mem' ->
+            find default_impl
+            implementing (pred default)
+            with-locals (map.put (map.put locals err (word.of_Z 1))
+                              var garbage)
+            and-memory mem' and-trace tr and-rest R
+            and-functions functions) ->
+        (let head := v in
+         find (cmd.seq
+                 (cmd.call [err; var] (fst (@KVStore.get ops)) [expr.var m_var; expr.var k_var])
+                 (cmd.cond (expr.op bopname.eq (expr.var err) (expr.literal 0))
+                           K_impl
+                           default_impl))
+         implementing (pred (do_or_default head K default))
+         with-locals locals and-memory mem and-trace tr and-rest R
+         and-functions functions).
+    Proof.
+      intros.
+      repeat straightline.
+      exists [m_ptr; k_ptr].
+      split.
+      { cbn.
+        eexists; split; [ eassumption | ].
+        eexists; split; [ eassumption | ].
+        reflexivity. }
+      kv_hammer.
+      destruct_one_match_hyp_of_type (option (annotation * value)).
+      { destruct_products.
+        destruct_one_match_hyp_of_type annotation; try contradiction.
+        subst. subst m. subst v.
+        match goal with
+        | l := context [map.put _ err] |- _ => subst l
+        end.
+        erewrite get_deannotate_Some by eassumption.
+        cbn [do_or_default].
+        exists (word.of_Z 1).
+        split.
+        { eexists.
+          split.
+          { rewrite ?map.get_put_diff, map.get_put_same by congruence.
+            reflexivity. }
+          { reflexivity. } }
+        { rewrite word.unsigned_of_Z_1.
+          split; try congruence; [ ]. intros.
+          cbn [fst snd].
+          match goal with
+          | H : _ |- _ => apply H
+          end.
+          { erewrite get_deannotate_Some by eassumption.
+            reflexivity. }
+          { ecancel_assumption. } } }
+      { destruct_products.
+        subst. subst m. subst v.
+        match goal with
+        | l := context [map.put _ err] |- _ => subst l
+        end.
+        erewrite get_deannotate_None by eassumption.
+        cbn [do_or_default].
+        exists (word.of_Z 0).
+        split.
+        { eexists.
+          split.
+          { rewrite ?map.get_put_diff, map.get_put_same by congruence.
+            reflexivity. }
+          { reflexivity. } }
+        { rewrite word.unsigned_of_Z_0.
+          split; try congruence; [ ]. intros.
+          cbn [fst snd].
+          match goal with
+          | H : _ |- _ => apply H
+          end.
+          { eapply get_deannotate_None. eassumption. }
+          { ecancel_assumption. } } }
+    Qed.
+
+    Derive kvswap_body SuchThat
+           (let kvswap := ("kvswap", (["m"; "k1"; "k2"], [],
+                                      kvswap_body)) in
+            program_logic_goal_for kvswap
+            (forall functions,
+                forall pm m pk1 k1 pk2 k2 R tr mem,
+                  k1 <> k2 -> (* TODO: try removing *)
+                  (Map pm m * Key pk1 k1 * Key pk2 k2 * R)%sep mem ->
+                  WeakestPrecondition.call
+                    (kvswap :: functions)
+                    "kvswap"
+                    tr mem [pm; pk1; pk2]
+                    (postcondition_for
+                       (MapAndTwoKeys
+                          pm pk1 pk2
+                          (kvswap_gallina m k1 k2)) R tr)))
+        As kvswap_body_correct.
+    Proof.
+        setup.
+        add_map_annotations.
+        eapply compile_map_get with (var:="v1") (err:="err") (M:=annotate m).
+        all:repeat t.
+    Admitted.
 End GallinaIncr.
